fstar/MLS.Crypto.Derived.fsti
@@ -8,8 +8,11 @@ open MLS.Result
 val available_ciphersuite_from_network: cipher_suite_nt -> result available_ciphersuite
 val available_ciphersuite_to_network: available_ciphersuite -> cipher_suite_nt
 
-val sign_with_label: #bytes:Type0 -> {|crypto_bytes bytes|} -> signature_key:sign_private_key bytes -> label:bytes -> content:bytes -> entropy:sign_nonce bytes -> result (sign_signature bytes)
-val verify_with_label: #bytes:Type0 -> {|crypto_bytes bytes|} -> verification_key:sign_public_key bytes -> label:bytes -> content:bytes -> signature:sign_signature bytes -> result bool
+let valid_label = s:string{b2t (normalize_term (string_is_ascii s)) /\ normalize_term (String.length s) < normalize_term ((pow2 30) - 8)}
+
+val sign_with_label_pre: #bytes:Type0 -> {|crypto_bytes bytes|} -> valid_label -> mls_bytes bytes -> bool
+val sign_with_label: #bytes:Type0 -> {|crypto_bytes bytes|} -> signature_key:sign_private_key bytes -> label:valid_label -> content:mls_bytes bytes{sign_with_label_pre #bytes label content} -> entropy:sign_nonce bytes -> sign_signature bytes
+val verify_with_label: #bytes:Type0 -> {|crypto_bytes bytes|} -> verification_key:sign_public_key bytes -> label:valid_label -> content:mls_bytes bytes{sign_with_label_pre #bytes label content} -> signature:sign_signature bytes -> bool
 
 val expand_with_label: #bytes:Type0 -> {|crypto_bytes bytes|} -> secret:bytes -> label:bytes -> context:bytes -> len:nat -> result (lbytes bytes len)
 val derive_secret: #bytes:Type0 -> {|crypto_bytes bytes|} -> secret:bytes -> label:bytes -> result (lbytes bytes (kdf_length #bytes))
