fstar/MLS.TreeDEM.Welcome.fst
@@ -333,7 +333,6 @@ let encrypt_welcome #bytes #cb group_info joiner_secret key_packages rand =
     let group_info_bytes = serialize (group_info_nt bytes) group_info_network in
     aead_encrypt welcome_key welcome_nonce empty group_info_bytes
   );
-  bytes_length_nil #bytes ps_pre_shared_key_id_nt;
   group_secrets <-- encrypt_group_secrets joiner_secret key_packages [] (*TODO psks*) rand;
   return ({
     secrets = group_secrets;
@@ -346,9 +345,12 @@ let encrypt_welcome #bytes #cb group_info joiner_secret key_packages rand =
 val sign_welcome_group_info: #bytes:Type0 -> {|crypto_bytes bytes|} -> sign_private_key bytes -> welcome_group_info bytes -> sign_nonce bytes -> result (welcome_group_info bytes)
 let sign_welcome_group_info #bytes #cb sign_sk gi rand =
   gi_network <-- welcome_group_info_to_network gi;
-  let tbs_bytes = serialize (group_info_tbs_nt bytes) gi_network.tbs in
-  signature <-- sign_with_label sign_sk (string_to_bytes #bytes "GroupInfoTBS") tbs_bytes rand;
-  return ({gi with signature = signature})
+  let tbs_bytes: bytes = serialize (group_info_tbs_nt bytes) gi_network.tbs in
+  if not (length tbs_bytes < pow2 30 && sign_with_label_pre #bytes "GroupInfoTBS" tbs_bytes) then error "sign_welcome_group_info: tbs too long"
+  else (
+    let signature = sign_with_label sign_sk "GroupInfoTBS" tbs_bytes rand in
+    return ({gi with signature = signature})
+  )
 
 val verify_welcome_group_info: #bytes:Type0 -> {|crypto_bytes bytes|} -> (nat -> result (sign_public_key bytes)) -> welcome_group_info bytes -> result bool
 let verify_welcome_group_info #bytes #cb get_sign_pk gi =
@@ -356,7 +358,8 @@ let verify_welcome_group_info #bytes #cb get_sign_pk gi =
     error "verify_welcome_group_info: bad signature size"
   else (
     gi_network <-- welcome_group_info_to_network gi;
-    let tbs_bytes = serialize (group_info_tbs_nt bytes) gi_network.tbs in
     sign_pk <-- get_sign_pk gi.signer;
-    verify_with_label sign_pk (string_to_bytes #bytes "GroupInfoTBS") tbs_bytes gi.signature
+    let tbs_bytes: bytes = serialize (group_info_tbs_nt bytes) gi_network.tbs in
+    if not (length tbs_bytes < pow2 30 && sign_with_label_pre #bytes "GroupInfoTBS" tbs_bytes) then error "sign_welcome_group_info: tbs too long"
+    else return (verify_with_label sign_pk "GroupInfoTBS" tbs_bytes gi.signature)
   )
